src/program_proof/examples/async_mem_alloc_dir_proof.v
@@ -667,7 +667,6 @@ Section goose.
     { crash_case. by iApply pre_inodes_to_cinv. }
     wpc_frame_seq.
     wp_apply (wp_NewMap unit (t:=struct.t alloc.unit)).
-    { apply unit_IntoValForType. }
     iIntros (addrs_ref) "Hused_set".
     iApply is_addrset_from_empty in "Hused_set".
     iNamed 1.
